Interpretations are represented by an ordered pair, $(p,q)$, where the first element is the truth value of p and the second the truth value of q.
\begin{enumerate}
    \item Mod($p \vee \neg p$) $= \{(T,T), (T,F), (F,T), (F,F)\}$

    \item Mod($p \vee q$) $= \{(T,T), (T,F), (F,T)\}$

    \item Mod($p \vee \neg q$) $= \{(T,T), (T,F), (F,F)\}$

    \item Mod($\neg p \vee q$) $= \{(T,T), (F,T), (F,F)\}$

    \item Mod($\neg p \vee \neg q$) $= \{(T,F), (F,T), (F,F)\}$

    \item Mod($p$) $= \{(T,T), (T,F)\}$

    \item Mod($q$) $= \{(T,T), (F,T)\}$

    \item Mod($p \leftrightarrow q$) $= \{(T,T), (F,F)\}$

    \item Mod($\neg (p \leftrightarrow q)$) $= \{(T,F), (F,T)\}$
    
    \item Mod($\neg q$) $= \{(T,F), (F,F)\}$

    \item Mod($\neg p$) $= \{(F,T), (F,F)\}$

    \item Mod($p \wedge q$) $= \{(T,T)\}$

    \item Mod($p \wedge \neg q$) $= \{(T,F)\}$

    \item Mod($\neg p \wedge q$) $= \{(F,T)\}$

    \item Mod($\neg p \wedge \neg q$) $= \{(F,F)\}$

    \item Mod($p \wedge \neg p$) $= \o$
\end{enumerate}