% {A ∧ B → C} |= (A → C) ∨ (B → C)
First consider:
\begin{align*}
    \{A \wedge B \rightarrow C\} &\Leftrightarrow \neg(A \wedge B) \vee C\\
    &\Leftrightarrow \neg A \vee \neg B \vee C
\end{align*}

Now consider:
\begin{align*}
    (A \rightarrow C) \vee (B \rightarrow C) &\Leftrightarrow \neg A \vee C \vee \neg B \vee C\\
    &\Leftrightarrow \neg A \vee \neg B \vee C
\end{align*}

So clearly:
\begin{align*}
    \{A \wedge B \rightarrow C\} \models (A \rightarrow C) \vee (B \rightarrow C)
\end{align*}

However consider below where (A,B,C) is an ordered tuple representing the respective truth values:
\begin{align*}
    (T,F,F), (T,F,T) \in \{A \wedge B \rightarrow C\}\\
    \text{But: } (T,F,F) \notin A \rightarrow C\\
    \text{Therefore: } \{A \wedge B \rightarrow C\} \nvDash A \rightarrow C\\
    \text{and}\\
    (F,T,F), (F,T,T) \in \{A \wedge B \rightarrow C\}\\
    \text{But: } (F,T,F) \notin B \rightarrow C\\
    \text{Therefore: } \{A \wedge B \rightarrow C\} \nvDash B \rightarrow C
\end{align*}